src/Utils2.fsti
@@ -58,26 +58,20 @@ let max64_nat : nat = FStar.Int.max_int U64.n
 noextract inline_for_extraction
 let max64 : U64.t = U64.lognot 0UL
 
+noextract
 let nth_is_zero (x: U64.t) (pos: U32.t{U32.v pos < 64})
   : bool
   = FU.nth (U64.v x) (U64.n - U32.v pos - 1) = false
 
-// CAUTION: assume val
-val ffs64 (x: U64.t)
-  : Pure U32.t
-  (requires U64.v x <> U64.v max64)
-  (ensures fun r ->
-    U32.v r < 64 /\
-    nth_is_zero x r
-  )
-
-val ffs64_ (x: U64.t) (bound: U32.t)
+module G = FStar.Ghost
+// CAUTION: assume val, no implementation
+val ffs64 (x: U64.t) (bound: G.erased U32.t)
   : Pure U32.t
   (requires
-    U32.v bound < 64 /\
-    (exists (k:nat{k < U32.v bound}). nth_is_zero x (U32.uint_to_t k)))
+    U32.v (G.reveal bound) < 64 /\
+    (exists (k:nat{k < U32.v (G.reveal bound)}). nth_is_zero x (U32.uint_to_t k)))
   (ensures fun r ->
-    U32.v r < U32.v bound /\
+    U32.v r < U32.v (G.reveal bound) /\
     nth_is_zero x r /\
     (forall (k:nat{k < U64.n /\ nth_is_zero x (U32.uint_to_t k)}).
       U32.v r <= k
